[micromega] Simplex uses alternatively Gomory cuts and case splits

plugins/micromega/certificate.ml
@@ -1134,7 +1134,6 @@ let rev_concat l =
   in
   conc [] l
 
-
 let pre_process sys =
   let sys = normalise sys in
   let bnd1 = bound_monomials sys in
